correct computational structure for systems of contracts, along with a strong notion of bisimulation.

theories/ContractSystems.v
@@ -15,67 +15,40 @@ From FinCert.Meta Require Import ContractMorphisms.
 
 Import ListNotations.
 
-(** Notation for a system of contracts, encoded as graphs, inspired by Milner's bigraphs *)
-
 Section ContractSystems.
 Context {Base : ChainBase}.
 
-(** First the node type *)
-(** The fundamental building block of a system: a contract and its address *)
-Section GeneralizedContract.
+Section LinkGraph.
 
-Record GeneralizedContract
-      (Setup Msg State Error : Type)
-      `{Serializable Setup}
-      `{Serializable Msg}
-      `{Serializable State}
-      `{Serializable Error} :=
-  build_gc_long {
-    gc_caddr : Address ;
-    gc_c : Contract Setup Msg State Error ;
-  }.
-
-Definition gc_caddr' 
-    {Setup Msg State Error : Type}
-    `{Serializable Setup}
-    `{Serializable Msg}
-    `{Serializable State}
-    `{Serializable Error}
-    (gc : GeneralizedContract Setup Msg State Error) := 
-    gc_caddr Setup Msg State Error gc.
-
-Definition gc_c' 
-    {Setup Msg State Error : Type}
-    `{Serializable Setup}
-    `{Serializable Msg}
-    `{Serializable State}
-    `{Serializable Error}
-    (gc : GeneralizedContract Setup Msg State Error) := 
-    gc_c Setup Msg State Error gc.
-
-Definition build_gc 
-    {Setup Msg State Error : Type}
-    `{ser_set : Serializable Setup}
-    `{ser_msg : Serializable Msg}
-    `{ser_st : Serializable State}
-    `{ser_err : Serializable Error}
-    (caddr : Address)
-    (C : Contract Setup Msg State Error) := 
-    build_gc_long Setup Msg State Error ser_set ser_msg ser_st ser_err caddr C.
-
-End GeneralizedContract.
-
-
-(** The Place Graph *)
-Section PlaceGraph.
-
-(* an inductive definition of trees *)
-Section NTree.
+Section ntree.
 
 Inductive ntree (T : Type) : Type :=
 | Node : T -> list (ntree T) -> ntree T.
 
-(** Utils *)
+Definition singleton_ntree {T} (t : T) := Node T t nil.
+
+(* fold/traversal for ntrees *)
+Fixpoint ntree_fold_left {A T}
+    (f : A -> T -> A)
+    (sys : ntree T)
+    (a0 : A) : A := 
+    match sys with 
+    | Node _ t list_child_trees => 
+        List.fold_left
+            (fun (a0' : A) (sys' : ntree T) =>
+                ntree_fold_left f sys' a0')
+            list_child_trees
+            (f a0 t)
+    end.
+
+(* ntree map : the functoriality of ntrees *)
+Fixpoint ntree_map {T T'} (f : T -> T') (tree : ntree T) : ntree T' := 
+    match tree with
+    | Node _ v children => 
+        Node T' (f v) (List.map (fun child => ntree_map f child) children)
+    end.
+
+(* WRONG *)
 Fixpoint replace_at_index {T : Type} (n : nat) (new_elem : T) (l : list T) : list T :=
   match l, n with
   | nil, _ => nil
@@ -83,18 +56,7 @@ Fixpoint replace_at_index {T : Type} (n : nat) (new_elem : T) (l : list T) : lis
   | hd :: tl, S n' => hd :: replace_at_index n' new_elem tl
   end.
 
-(* Update a tree at a given index, which can be at a node or a leaf *)
-Fixpoint update_ntree_at_index {T : Type} (tree : ntree T) (value : T) (leaf_index : list nat) : ntree T :=
-  match tree, leaf_index with
-  | Node _ v children, nil => Node T value children (* Reached the desired leaf *)
-  | Node _ v children, i :: is =>
-      match List.nth_error children i with
-      | Some child => Node T v (replace_at_index i (update_ntree_at_index child value is) children)
-      | None => tree (* Invalid leaf index *)
-      end
-  end.
-
-(* Merge semantics: add a tree to a given leaf *)
+(* WRONG *)
 Fixpoint add_tree_at_leaf {T} (orig append : ntree T) (leaf_index : list nat) : ntree T :=
     match orig, leaf_index with
     | Node _ v children, nil => orig (* Must add only at a leaf *)
@@ -105,944 +67,1048 @@ Fixpoint add_tree_at_leaf {T} (orig append : ntree T) (leaf_index : list nat) : 
         end
     end.
 
-Fixpoint ntree_find_node {T} (leaf_index : list nat) (tree : ntree T) : option T :=
-    match tree, leaf_index with 
-    | Node _ v children, nil => Some v (* Reached the desired node *)
-    | Node _ v children, i :: is =>
-        match List.nth_error children i with
-        | Some child => ntree_find_node is child (* Iterate *)
-        | None => None (* Invalid leaf index *)
-        end
-    end.
+End ntree.
 
-(* Definition empty_ntree {T} := Leaf T. *)
-
-Definition singleton_ntree {T} (t : T) := Node T t nil.
-
-Definition in_ntree {T} (t : T) (tree : ntree T) : Prop := 
-    exists leaf_index, ntree_find_node leaf_index tree = Some t.
-
-Definition search_ntree {T} (t : T) (tree : ntree T) : bool.
-Admitted.
-
-(* Given an accumulating function and a starting point, iterate over the tree *)
-Fixpoint ntree_accum {T} (tree : ntree T) (accum : T -> T -> T) (t : T) : T :=
-    match tree with 
-    | Node _ v children => 
-        List.fold_left 
-        (fun (t' : T) (child : ntree T) => accum (ntree_accum child accum t) t')
-        children
-        (accum v t)
-    end.
-
-(** Functoriality *)
-Fixpoint ntree_funct {T T'} (f : T -> T') (tree : ntree T) : ntree T' := 
-    match tree with 
-    | Node _ v children => 
-        Node T' (f v) (List.map (fun child => ntree_funct f child) children)
-    end.
-
-(* TODO Will need to make own induction principle it looks like 
-Lemma ntree_find_funct {T T'} (f : T -> T') (index : list nat) (tree : ntree T) : 
-    ntree_find_node index (ntree_funct f tree) = 
-    option_map f (ntree_find_node index tree).
-Proof.
-    destruct tree, index; auto.
-    unfold ntree_find_node.
-    simpl.
-    rewrite nth_error_map.
-    induction (nth_error l n); auto.
-    cbn.
-Admitted.
-
-Lemma ntree_update_funct {T T'} (f : T -> T') index t tree : 
-    update_ntree_at_index (ntree_funct f tree) (f t) index = 
-    ntree_funct f (update_ntree_at_index tree t index).
-Admitted.
-
-Lemma in_ntree_funct {T T'} (f : T -> T') t tree :
-    in_ntree t tree -> in_ntree (f t) (ntree_funct f tree).
-Proof.
-    intro in_tree.
-    destruct in_tree as [index is_in].
-    unfold in_ntree.
-    exists index.
-    rewrite ntree_find_funct.
-    now rewrite is_in.
-Qed.
-*)
-
-(** Permutations *)
-Inductive NTree_Permutation {T} : ntree T -> ntree T -> Prop := 
-| perm_swap v children1 children2 :
-    Permutation children1 children2 ->
-    NTree_Permutation (Node T v children1) (Node T v children2)
-| perm_trans ntree1 ntree2 ntree3 : 
-    NTree_Permutation ntree1 ntree2 ->
-    NTree_Permutation ntree2 ntree3 ->
-    NTree_Permutation ntree1 ntree3.
-
-Lemma ntree_permutation_comm {T} (ntree1 ntree2 : ntree T) : 
-    NTree_Permutation ntree1 ntree2 -> 
-    NTree_Permutation ntree2 ntree1.
-Proof.
-    intro perm.
-    induction perm.
-    -   apply Permutation_sym in H.
-        now apply perm_swap.
-    -   apply (perm_trans ntree3 ntree2 ntree1 IHperm2 IHperm1).
-Qed.
-
-(*
-Lemma intree_permutation_in {T}
-    t (ntree1 ntree2 : ntree T) :
-    NTree_Permutation ntree1 ntree2 ->
-    (in_ntree t ntree1 <-> in_ntree t ntree2).
-Proof.
-    intro perm.
-    induction perm; auto;
-    split.
-    (* -> *)
-    -   intro H_in1.
-        unfold in_ntree in *.
-        destruct H_in1 as [place found].
-        destruct place eqn:H_place.
-        +   cbn in found.
-            inversion found.
-            now exists nil.
-        +   destruct H eqn:H_perm.
-            cbn in found.
-            *   destruct n; cbn in found; inversion found.
-            *   admit.      
-            *   admit.
-            *   admit.
-    (* <- *)
-    -   admit.
-Admitted.
-*)
-
-End NTree.
-
-End PlaceGraph.
-
-(** A system of contracts is a (list of) place graphs, 
-    endowed automatically with the link graph structure *)
-Section SystemDefinition.
-
-(* A system of contracts is presented by its place graph;
-    it inherits the link graph automatically *)
 Definition ContractSystem
-    (Setup Msg State : Type)
+    (Setup Msg State Error : Type)
     `{sys_set : Serializable Setup}
     `{sys_msg : Serializable Msg}
-    `{sys_st : Serializable State} :=
-    ntree (GeneralizedContract Setup Msg State nat).
+    `{sys_st  : Serializable State}
+    `{sys_err : Serializable Error} :=
+    ntree (Contract Setup Msg State Error).
 
-(* An iterative construction of a system of contracts *)
-Section GC_Iter.
-
-Section GC_Sum.
-Context `{Serializable Setup1} `{Serializable Msg1} `{Serializable State1}
-        `{Serializable Setup2} `{Serializable Msg2} `{Serializable State2}.
-
-Definition c_to_c_sum_l (C : Contract Setup1 Msg1 State1 nat) :
-    Contract (Setup1 + Setup2) (Msg1 + Msg2) (State1 + State2) nat.
-Proof.
-    destruct C as [init1 recv1].
-    apply build_contract.
-    (* init *)
-    -   exact (fun c ctx s' =>
-            match s' with
-            | inl s =>
-                match init1 c ctx s with
-                | Ok st => Ok (inl st)
-                | Err e => Err e
-                end
-            | inr _ => Err 0
-            end).
-    (* receive *)
-    -   exact (fun c ctx st' op_msg' =>
-            match st', op_msg' with 
-            | inl st, Some (inl msg) => 
-                match recv1 c ctx st (Some msg) with 
-                | Ok (new_st, acts) => Ok (inl new_st, acts)
-                | Err e => Err e
-                end
-            | inl st, None => 
-                match recv1 c ctx st None with 
-                | Ok (new_st, acts) => Ok (inl new_st, acts)
-                | Err e => Err e
-                end
-            | _ , _ => Err 0
-            end).
-Defined.
-
-Definition gc_to_gc_sum_l (sys : GeneralizedContract Setup1 Msg1 State1 nat) :
-    GeneralizedContract (Setup1 + Setup2) (Msg1 + Msg2) (State1 + State2) nat := 
-    {| gc_caddr := (gc_caddr' sys) ; 
-       gc_c := c_to_c_sum_l (gc_c' sys) ; |}.
-
-Definition c_to_c_sum_r (C : Contract Setup1 Msg1 State1 nat) :
-    Contract (Setup2 + Setup1) (Msg2 + Msg1) (State2 + State1) nat.
-Proof.
-    destruct C as [init1 recv1].
-    apply build_contract.
-    (* init *)
-    -   exact (fun c ctx s' => 
-            match s' with 
-            | inr s => 
-                match init1 c ctx s with 
-                | Ok st => Ok (inr st)
-                | Err e => Err e
-                end
-            | inl _ => Err 0
-            end).
-    (* receive *)
-    -   exact (fun c ctx st' op_msg' =>
-            match st', op_msg' with 
-            | inr st, Some (inr msg) => 
-                match recv1 c ctx st (Some msg) with 
-                | Ok (new_st, acts) => Ok (inr new_st, acts)
-                | Err e => Err e
-                end
-            | inr st, None => 
-                match recv1 c ctx st None with 
-                | Ok (new_st, acts) => Ok (inr new_st, acts)
-                | Err e => Err e
-                end
-            | _ , _ => Err 0
-            end).
-Defined.
-
-Definition gc_to_gc_sum_r (sys : GeneralizedContract Setup1 Msg1 State1 nat) :
-    GeneralizedContract (Setup2 + Setup1) (Msg2 + Msg1) (State2 + State1) nat := 
-    {| gc_caddr := (gc_caddr' sys) ; 
-       gc_c := c_to_c_sum_r (gc_c' sys) ; |}.
-
-End GC_Sum.
-
-
-Context `{Serializable Setup1} `{Serializable Msg1} 
-        `{Serializable State1} `{Serializable Error1}
-        `{Serializable Setup2} `{Serializable Msg2} 
-        `{Serializable State2} `{Serializable Error2}.
-
-Definition singleton_sys 
-    `{Serializable Setup} `{Serializable Msg} `{Serializable State}
-    (gc : GeneralizedContract Setup Msg State nat) 
-    : ContractSystem Setup Msg State := 
-    singleton_ntree gc.
-
-Definition build_system_iter
-    (sys : ContractSystem Setup1 Msg1 State1)
-    (leaf_index : list nat)
-    (G2 : GeneralizedContract Setup2 Msg2 State2 nat)
-    : ContractSystem (Setup1 + Setup2) (Msg1 + Msg2) (State1 + State2) :=
-        add_tree_at_leaf
-        (ntree_funct gc_to_gc_sum_l sys)
-        (singleton_sys (gc_to_gc_sum_r (build_gc (gc_caddr' G2) (gc_c' G2))))
-        leaf_index.
-
-(* For convenience, to nest one contract inside another *)
-Definition nest 
-    (outer : GeneralizedContract Setup1 Msg1 State1 nat) 
-    (inner : GeneralizedContract Setup2 Msg2 State2 nat)
-    : ContractSystem (Setup1 + Setup2) (Msg1 + Msg2) (State1 + State2) :=
-    build_system_iter
-        (singleton_sys outer)
-        [0]
-        inner.
-
-End GC_Iter.
-
-
-(** A system is defined by its collective state and interface,
-    from which we can get a system `receive` function *)
 Section SystemInterface.
+Context `{Serializable Setup} `{Serializable Msg} `{Serializable State} `{Serializable Error}.
 
-(** System state *)
-Definition SystemState (State : Type) : Type := ntree (option State).
-
-(** System interface *)
-Record SystemMsg (Msg : Type) `{Serializable Msg} := {
-    sm_msg : option Msg ;
-    sm_place : list nat ; (* the index of *which* contract gets called *)
-}.
-
-Definition sm_msg' `{Serializable Msg} (sm : SystemMsg Msg) := sm_msg Msg sm.
-Definition sm_place' `{Serializable Msg} (sm : SystemMsg Msg) := sm_place Msg sm.
-
-(* Move from System State to System State *)
-Definition sys_receive 
-    {Setup Msg State : Type}
-    `{sys_set : Serializable Setup}
-    `{sys_msg : Serializable Msg}
-    `{sys_st : Serializable State}
-    (sys : ContractSystem Setup Msg State)
+(* system init : just initialize the root, since all contract init behaves identically *)
+Definition sys_init
+    (sys : ContractSystem Setup Msg State Error)
     (c : Chain)
     (ctx : ContractCallContext)
-    (sys_st : SystemState State) (* state *)
-    (sys_msg : SystemMsg Msg) (* message *) :
-    result (SystemState State * list ActionBody) nat := 
-    match ntree_find_node (sm_place' sys_msg) sys with 
-    | Some gc => 
-        match ntree_find_node (sm_place' sys_msg) sys_st with 
-        | Some st_op => 
-            match st_op with 
-            | Some st => 
-                match receive (gc_c' gc) c ctx st (sm_msg' sys_msg) with 
-                | Ok (new_st, new_acts) =>
-                    let new_sys_st := 
-                    update_ntree_at_index sys_st (Some new_st) (sm_place' sys_msg) in
-                    Ok (new_sys_st, new_acts)
+    (s : Setup) : result State Error := 
+    match sys with 
+    | Node _ root_contract _ => 
+        init root_contract c ctx s 
+    end.
+
+(* system receive: take the message and state and run through the entire system.
+    since systems are iteratively built so that a message not intended for a given contract 
+    returns the identity, this targets the contract in question and leaves the rest untouched. *)
+Definition sys_receive
+    (sys : ContractSystem Setup Msg State Error)
+    (c : Chain)
+    (ctx : ContractCallContext)
+    (st : State)
+    (op_msg : option Msg) : result (State * list ActionBody) Error :=
+    ntree_fold_left
+    (fun (recv_propogate : result (State * list ActionBody) Error)
+         (contr : Contract Setup Msg State Error) =>
+         match recv_propogate with 
+            | Ok (st0, lacts0) => 
+                match receive contr c ctx st0 op_msg with 
+                | Ok (st1, lacts1) => Ok (st1, lacts0 ++ lacts1)
                 | Err e => Err e
                 end
-            | None => Err 0
-            end
-        | None => Err 0
-        end
-    | None => Err 0
-    end.
+            | Err e => Err e
+         end)
+    sys
+    (Ok (st, nil)).
+
+(* thes two functions give us a contract *)
+Definition sys_contract (sys : ContractSystem Setup Msg State Error) := 
+    build_contract (sys_init sys) (sys_receive sys).
 
 End SystemInterface.
 
-End SystemDefinition.
 
+Section IterativeSystemBuild.
+(* the definition of a singleton system *)
+Definition singleton_sys 
+    `{Serializable Setup} `{Serializable Msg} `{Serializable State} `{Serializable Error}
+    (C : Contract Setup Msg State Error) 
+    : ContractSystem Setup Msg State Error := singleton_ntree C.
 
-(** The Link Graph *)
-Section LinkGraph.
+Section IterativeSum.
+Context `{Serializable Setup1} `{Serializable Msg1} `{Serializable State1} `{Serializable Error1}
+        `{Serializable Setup2} `{Serializable Msg2} `{Serializable State2} `{Serializable Error2}.
 
-(* the system's graph *)
-Definition call_to call : option Address := 
-    match call with 
-    | act_transfer _ _ => None 
-    | act_call caddr _ _ => Some caddr 
-    | act_deploy _ _ _ => None 
+(* an iterative add to contract systems s.t. type goals are satisfied *)
+
+(* accepts messages on the left *)
+Definition c_sum_l
+    (C1 : Contract Setup1 Msg1 State1 Error1)
+    (C2 : Contract Setup2 Msg2 State2 Error2) :
+    Contract (Setup1 * Setup2) (Msg1 + Msg2) (State1 * State2) (Error1 + Error2).
+Proof.
+    destruct C1 as [init1 recv1].
+    destruct C2 as [init2 recv2].
+    apply build_contract.
+    (* each setup must succeed, providing the new system state *)
+    -   apply (fun c ctx s' => 
+            let '(s1, s2) := s' in
+            match init1 c ctx s1, init2 c ctx s2 with 
+            | Ok st1, Ok st2 => Ok (st1, st2)
+            | Err e, _ => Err (inl e) (* the left error is first *)
+            | _, Err e => Err (inr e) (* followed by the right *)
+            end).
+    -   apply (fun c ctx st' op_msg => 
+            let '(st1, st2) := st' in
+            match op_msg with 
+            | Some msg => 
+                match msg with 
+                (* the message was intended for this contract, 
+                    so we attempt to udpate the state *)
+                | inl msg =>
+                    match recv1 c ctx st1 (Some msg) with 
+                    | Ok (new_st1, nacts) => Ok ((new_st1, st2), nacts)
+                    | Err e => Err (inl e)
+                    end
+                (* the message was not intended for this contract, so we do nothing *)
+                | inr msg => Ok (st', nil)
+                end 
+            | None => (* ? maybe just the id? *)
+                Ok (st', nil)
+            end).
+Defined.
+
+(* same as before, but accepts messages on the right now *)
+Definition c_sum_r 
+    (C1 : Contract Setup1 Msg1 State1 Error1)
+    (C2 : Contract Setup2 Msg2 State2 Error2) :
+    Contract (Setup1 * Setup2) (Msg1 + Msg2) (State1 * State2) (Error1 + Error2).
+Proof.
+    destruct C1 as [init1 recv1].
+    destruct C2 as [init2 recv2].
+    apply build_contract.
+    (* each setup must succeed, providing the new system state *)
+    -   apply (fun c ctx s' =>
+            let '(s1, s2) := s' in
+            match init1 c ctx s1, init2 c ctx s2 with
+            | Ok st1, Ok st2 => Ok (st1, st2)
+            | Err e, _ => Err (inl e) (* the left error is first *)
+            | _, Err e => Err (inr e) (* followed by the right *)
+            end).
+    -   apply (fun c ctx st' op_msg =>
+            let '(st1, st2) := st' in
+            match op_msg with
+            | Some msg =>
+                match msg with
+                (* the message was not intended for this contract, so we do nothing *)
+                | inl msg => Ok (st', nil)
+                (* the message was intended for this contract, 
+                    so we attempt to udpate the state *)
+                | inr msg =>
+                    match recv2 c ctx st2 (Some msg) with 
+                    | Ok (new_st2, nacts) => Ok ((st1, new_st2), nacts)
+                    | Err e => Err (inr e)
+                    end
+                end
+            | None => (* ? maybe just the id? *)
+                Ok (st', nil)
+            end).
+Defined.
+
+End IterativeSum.
+
+Section IterativeChild.
+Context `{Serializable Setup1} `{Serializable Msg1} `{Serializable State1} `{Serializable Error1}
+        `{Serializable Setup2} `{Serializable Msg2} `{Serializable State2} `{Serializable Error2}.
+
+(* add a contract as a child to a system(/nest contracts) *)
+Definition sys_add_child_r
+    (sys : ContractSystem Setup1 Msg1 State1 Error1)
+    (C : Contract Setup2 Msg2 State2 Error2) :
+    ContractSystem (Setup1 * Setup2) (Msg1 + Msg2) (State1 * State2) (Error1 + Error2) := 
+    let T := (Contract (Setup1 * Setup2) (Msg1 + Msg2) (State1 * State2) (Error1 + Error2)) in 
+    match sys with
+    | Node _ root_contract _ =>
+        match (ntree_map (fun C1 => c_sum_l C1 C) sys) with
+        | Node _ root_contract' children =>
+            Node T root_contract' (children ++ [Node T (c_sum_r root_contract C) nil])
+        end
     end.
 
-(* The type of edges *)
-(* Edges in the link graph are given by contract calls *)
-Record LinkGraphEdges 
-    `{Serializable Setup1} `{Serializable Msg1} `{Serializable State1} `{Serializable Error1}
-    `{Serializable Setup2} `{Serializable Msg2} `{Serializable State2} `{Serializable Error2}
-    (G1 : GeneralizedContract Setup1 Msg1 State1 Error1)
-    (G2 : GeneralizedContract Setup2 Msg2 State2 Error2) : Type := {
-    e_chain : Chain ;
-    e_ctx : ContractCallContext ;
-    e_prvstate : State1 ; (* prev state *)
-    e_msg : option Msg1 ; (* msg *)
-    e_newstate : State1 ; (* new state *)
-    e_nacts : list ActionBody ;
-    linking_act : ActionBody ; (* the action that links the two contracts *)
-    (* there is some transaction for which G1 calls G2 *)
-    e_recv_some : 
-        (* this is a successful call *)
-        receive (gc_c' G1) e_chain e_ctx e_prvstate e_msg = Ok (e_newstate, e_nacts) /\
-        (* which emits the transaction linking_act, *)
-        List.In linking_act e_nacts /\
-        (* and it is a call to G2 *)
-        call_to linking_act = Some (gc_caddr' G2) ;
-}.
+Definition nest 
+    (C1 : Contract Setup1 Msg1 State1 Error1)
+    (C2 : Contract Setup2 Msg2 State2 Error2) : 
+    ContractSystem (Setup1 * Setup2) (Msg1 + Msg2) (State1 * State2) (Error1 + Error2) := 
+    let T := (Contract (Setup1 * Setup2) (Msg1 + Msg2) (State1 * State2) (Error1 + Error2)) in 
+    Node T (c_sum_l C1 C2) [Node T (c_sum_r C1 C2) nil].
 
-(* edges can be composed if they are sequential transactions *)
-Definition edges_compose 
-    `{Serializable Setup1} `{Serializable Msg1} `{Serializable State1} `{Serializable Error1}
-    `{Serializable Setup2} `{Serializable Msg2} `{Serializable State2} `{Serializable Error2}
-    `{Serializable Setup3} `{Serializable Msg3} `{Serializable State3} `{Serializable Error3}
-    {G1 : GeneralizedContract Setup1 Msg1 State1 Error1}
-    {G2 : GeneralizedContract Setup2 Msg2 State2 Error2}
-    {G3 : GeneralizedContract Setup3 Msg3 State3 Error3}
-    (e1 : LinkGraphEdges G1 G2) (e2 : LinkGraphEdges G2 G3) : Prop := 
-    match linking_act G1 G2 e1 with 
-    | act_call _ _ msg => option_map serialize (e_msg G2 G3 e2) = Some msg
-    | _ => False
-    end.
+End IterativeChild.
+
+End IterativeSystemBuild.
 
 End LinkGraph.
 
 
-(** Contract System Utils *)
-Section SystemUtils.
+Section PlaceGraph.
+(* not sure what to make of this *)
+(* (TODO?) COMPOSE SEMANTICS of LINK and PLACE GRAPHS? *)
 
-(* get a system state from a bstate *)
-Definition sys_bstate
-    `{sys_set : Serializable Setup}
-    `{sys_msg : Serializable Msg}
-    `{sys_st : Serializable State}
-    (bstate : ChainState)
-    (sys : ContractSystem Setup Msg State) 
-    : SystemState SerializedValue :=
-    ntree_funct
-    (fun (gc : GeneralizedContract Setup Msg State nat) =>
-        env_contract_states bstate (gc_caddr' gc))
-    sys.
-
-Definition is_sys_state
-    `{sys_set : Serializable Setup}
-    `{sys_msg : Serializable Msg}
-    `{sys_st : Serializable State}
-    (bstate : ChainState)
-    (sys : ContractSystem Setup Msg State)
-    (sys_state : SystemState State) : Prop :=
-    forall place gc,
-    ntree_find_node place sys = Some gc <->
-    exists st_op,
-    ntree_find_node place sys_state = Some st_op /\
-    env_contract_states bstate (gc_caddr' gc) = option_map serialize st_op.
-
-(* a system is deployed *)
-Definition sys_deployed bstate
-    `{sys_set : Serializable Setup}
-    `{sys_msg : Serializable Msg}
-    `{sys_st : Serializable State}
-    (sys : ContractSystem Setup Msg Setup) : Prop :=
-    forall G,
-    in_ntree G sys ->
-    env_contracts bstate (gc_caddr' G) = Some (gc_c' G : WeakContract).
-
-(* the notion of the initial state of a system *)
-Definition is_genesis_state 
-    `{sys_set : Serializable Setup}
-    `{sys_msg : Serializable Msg}
-    `{sys_st : Serializable State}
-    `{sys_err : Serializable Error}
-    (C : Contract Setup Msg State Error) init_cstate : Prop := 
-    exists init_chain init_ctx init_setup, 
-    init C init_chain init_ctx init_setup = Ok init_cstate.
-
-(* a better version of this perhaps? *)
-Definition is_genesis_gstate_sys 
-    `{sys_set : Serializable Setup}
-    `{sys_msg : Serializable Msg}
-    `{sys_st : Serializable State}
-    (sys : ContractSystem Setup Msg State) gstate : Prop :=
-    forall place,
-    ((exists G, ntree_find_node place sys = Some G) <->
-     (exists st, ntree_find_node place gstate = Some (Some st))) /\
-    (forall place G st, 
-        ntree_find_node place sys = Some G ->
-        ntree_find_node place gstate = Some (Some st) ->
-        is_genesis_state (gc_c' G) st).
-
-(* some propositions relating to system morphisms *)
-Definition sys_genesis_prop
-    `{Serializable Setup1}
-    `{Serializable Msg1}
-    `{Serializable State1}
-    `{Serializable Setup2}
-    `{Serializable Msg2}
-    `{Serializable State2}
-    (sys1 : ContractSystem Setup1 Msg1 State1)
-    (sys2 : ContractSystem Setup2 Msg2 State2)
-    (gstate_morph : SystemState State1 -> SystemState State2) : Prop :=
-    forall gstate,
-        is_genesis_gstate_sys sys1 gstate ->
-        is_genesis_gstate_sys sys2 (gstate_morph gstate).
-
-Definition sys_coherence_prop
-    `{Serializable Setup1}
-    `{Serializable Msg1}
-    `{Serializable State1}
-    `{Serializable Setup2}
-    `{Serializable Msg2}
-    `{Serializable State2}
-    (sys1 : ContractSystem Setup1 Msg1 State1)
-    (sys2 : ContractSystem Setup2 Msg2 State2)
-    (gstate_morph : SystemState State1 -> SystemState State2)
-    (gmsg_morph : SystemMsg Msg1 -> SystemMsg Msg2)
-    (gerror_morph : nat -> nat) : Prop :=
-    forall c ctx gst gmsg,
-        result_functor (fun '(gst, l) => (gstate_morph gst, l)) gerror_morph
-            (sys_receive sys1 c ctx gst gmsg) =
-        sys_receive sys2 c ctx (gstate_morph gst) (gmsg_morph gmsg).
-
-End SystemUtils.
+End PlaceGraph.
 
 
-(** Morphisms, including isomorphisms, of contract systems *)
 Section SystemMorphism.
 
-Section MorphDefn.
-Context `{Serializable Setup1}
-        `{Serializable Msg1}
-        `{Serializable State1}
-        `{Serializable Setup2}
-        `{Serializable Msg2}
-        `{Serializable State2}
-        `{Serializable State1Accum}
-        `{Serializable State2Accum}.
+Section SystemMorphismDefinition.
+Context `{Serializable Setup1} `{Serializable Msg1} `{Serializable State1} `{Serializable Error1}
+        `{Serializable Setup2} `{Serializable Msg2} `{Serializable State2} `{Serializable Error2}.
+(* should imitate a contract morphism and be made with morphs of types 
+    with an init and recv coherence *)
 
-(* a morphism of systems of contracts *)
 Record SystemMorphism
-    (sys1 : ContractSystem Setup1 Msg1 State1)
-    (sys2 : ContractSystem Setup2 Msg2 State2) := 
-    build_sys_morphism {
-        (* component morphisms *)
-        gstate_morph : SystemState State1 -> SystemState State2 ;
-        gmsg_morph : SystemMsg Msg1 -> SystemMsg Msg2 ;
-        gerror_morph : nat -> nat ;
-        (* init coherence analogue *)
-        sys_genesis : forall gstate,
-            is_genesis_gstate_sys sys1 gstate ->
-            is_genesis_gstate_sys sys2 (gstate_morph gstate) ;
-        (* recv coherence analogue *)
-        sys_coherence : forall c ctx gst gmsg,
-            result_functor (fun '(gst, nacts) => (gstate_morph gst, nacts)) gerror_morph
-                (sys_receive sys1 c ctx gst gmsg) =
-            sys_receive sys2 c ctx (gstate_morph gst) (gmsg_morph gmsg) ;
+    (sys1 : ContractSystem Setup1 Msg1 State1 Error1) 
+    (sys2 : ContractSystem Setup2 Msg2 State2 Error2) := 
+    build_system_morphism {
+        (* the components of a morphism f *)
+        sys_setup_morph : Setup1 -> Setup2 ;
+        sys_msg_morph   : Msg1   -> Msg2   ;
+        sys_state_morph : State1 -> State2 ;
+        sys_error_morph : Error1 -> Error2 ;
+        (* coherence conditions *)
+        sys_init_coherence : forall c ctx s, 
+            result_functor sys_state_morph sys_error_morph 
+                (sys_init sys1 c ctx s) = 
+            sys_init sys2 c ctx (sys_setup_morph s) ;
+        sys_recv_coherence : forall c ctx st op_msg, 
+            result_functor (fun '(st, l) => (sys_state_morph st, l)) sys_error_morph 
+                (sys_receive sys1 c ctx st op_msg) = 
+            sys_receive sys2 c ctx (sys_state_morph st) (option_map sys_msg_morph op_msg) ; 
 }.
 
-End MorphDefn.
-
-Proposition eq_sm
-    `{Serializable Setup1}
-    `{Serializable Msg1}
-    `{Serializable State1}
-    `{Serializable Setup2}
-    `{Serializable Msg2}
-    `{Serializable State2}
-    {sys1 : ContractSystem Setup1 Msg1 State1}
-    {sys2 : ContractSystem Setup2 Msg2 State2}
-    (f g : SystemMorphism sys1 sys2) :
-    gstate_morph sys1 sys2 f = gstate_morph sys1 sys2 g -> 
-    gmsg_morph sys1 sys2 f = gmsg_morph sys1 sys2 g -> 
-    gerror_morph sys1 sys2 f = gerror_morph sys1 sys2 g -> 
-    f = g.
+(* a system morphism is in one-to-one correspondence with a morphism of contracts *)
+Definition cm_to_sysm
+    (sys1 : ContractSystem Setup1 Msg1 State1 Error1)
+    (sys2 : ContractSystem Setup2 Msg2 State2 Error2)
+    (f : ContractMorphism (sys_contract sys1) (sys_contract sys2)) : SystemMorphism sys1 sys2.
 Proof.
-    intros gst_eq gmsg_eq gerr_eq.
-    destruct f, g.
-    simpl in *.
-    subst.
-    f_equal; apply proof_irrelevance.
-Qed.
-
-Definition compose_sm
-    `{ser_setup1 : Serializable Setup1}
-    `{ser_msg1 : Serializable Msg1}
-    `{ser_state1 : Serializable State1}
-    `{ser_setup2 : Serializable Setup2}
-    `{ser_msg2 : Serializable Msg2}
-    `{ser_state2 : Serializable State2}
-    `{ser_setup3 : Serializable Setup3}
-    `{ser_msg3 : Serializable Msg3}
-    `{ser_state3 : Serializable State3}
-    {sys1 : ContractSystem Setup1 Msg1 State1}
-    {sys2 : ContractSystem Setup2 Msg2 State2}
-    {sys3 : ContractSystem Setup3 Msg3 State3}
-    (g : SystemMorphism sys2 sys3) (f : SystemMorphism sys1 sys2) : SystemMorphism sys1 sys3.
-Proof.
-    destruct g, f.
-    apply (build_sys_morphism sys1 sys3
-        (compose gstate_morph0 gstate_morph1)
-        (compose gmsg_morph0 gmsg_morph1)
-        (compose gerror_morph0 gerror_morph1)).
-    -   intros * is_gen.
-        now apply sys_genesis0, sys_genesis1.
-    -   intros.
-        cbn.
-        rewrite <- (sys_coherence0 c ctx (gstate_morph1 gst) (gmsg_morph1 gmsg)).
-        rewrite <- (sys_coherence1 c ctx gst gmsg).
-        unfold result_functor.
-        now destruct (sys_receive sys1 c ctx gst gmsg).
+    destruct f.
+    apply (build_system_morphism sys1 sys2 setup_morph msg_morph state_morph error_morph
+        init_coherence recv_coherence).
 Defined.
 
-Proposition compose_sm_assoc
-    `{ser_setup1 : Serializable Setup1}
-    `{ser_msg1 : Serializable Msg1}
-    `{ser_state1 : Serializable State1}
-    `{ser_setup2 : Serializable Setup2}
-    `{ser_msg2 : Serializable Msg2}
-    `{ser_state2 : Serializable State2}
-    `{ser_setup3 : Serializable Setup3}
-    `{ser_msg3 : Serializable Msg3}
-    `{ser_state3 : Serializable State3}
-    `{ser_setup4 : Serializable Setup4}
-    `{ser_msg4 : Serializable Msg4}
-    `{ser_state4 : Serializable State4}
-    {sys1 : ContractSystem Setup1 Msg1 State1}
-    {sys2 : ContractSystem Setup2 Msg2 State2}
-    {sys3 : ContractSystem Setup3 Msg3 State3}
-    {sys4 : ContractSystem Setup4 Msg4 State4}
-    (f : SystemMorphism sys1 sys2)
-    (g : SystemMorphism sys2 sys3)
+Definition sysm_to_cm
+    (sys1 : ContractSystem Setup1 Msg1 State1 Error1)
+    (sys2 : ContractSystem Setup2 Msg2 State2 Error2)
+    (f : SystemMorphism sys1 sys2) : ContractMorphism (sys_contract sys1) (sys_contract sys2).
+Proof.
+    destruct f as [sys_setup_morph sys_msg_morph sys_state_morph sys_error_morph sys_init_coh sys_recv_coh].
+    apply (build_contract_morphism (sys_contract sys1) (sys_contract sys2)
+        sys_setup_morph sys_msg_morph sys_state_morph sys_error_morph
+        sys_init_coh sys_recv_coh).
+Defined.
+
+Lemma cm_sysm_one_to_one
+    (sys1 : ContractSystem Setup1 Msg1 State1 Error1)
+    (sys2 : ContractSystem Setup2 Msg2 State2 Error2) :
+    compose (cm_to_sysm sys1 sys2) (sysm_to_cm sys1 sys2) = id /\
+    compose (sysm_to_cm sys1 sys2) (cm_to_sysm sys1 sys2) = id.
+Proof.
+    split; 
+    unfold sysm_to_cm, cm_to_sysm;
+    apply functional_extensionality;
+    intro;
+    now destruct x.
+Qed.
+
+End SystemMorphismDefinition.
+
+
+Section IdentitySystemMorphism.
+Context `{Serializable Msg} `{Serializable Setup} `{Serializable State} `{Serializable Error}.
+
+Lemma sys_init_coherence_id (sys : ContractSystem Setup Msg State Error) : 
+    forall c ctx s,
+    result_functor id id (sys_init sys c ctx s) = 
+    sys_init sys c ctx s.
+Proof. 
+    intros.
+    unfold result_functor.
+    now destruct (sys_init sys c ctx s).
+Qed.
+
+Lemma sys_recv_coherence_id (sys : ContractSystem Setup Msg State Error) :
+    forall c ctx st op_msg,
+    result_functor
+        (fun '(st, l) => (id st, l)) id
+        (sys_receive sys c ctx st op_msg) =
+    sys_receive sys c ctx (id st) (option_map id op_msg).
+Proof.
+    intros.
+    unfold result_functor, option_map.
+    cbn.
+    destruct op_msg.
+    -   now destruct (sys_receive sys c ctx st (Some m)); try destruct t.
+    -   now destruct (sys_receive sys c ctx st None); try destruct t.
+Qed.
+
+(** The identity morphism *)
+Definition id_sm (sys : ContractSystem Setup Msg State Error) : SystemMorphism sys sys := {|
+        (* components *)
+        sys_setup_morph := id ;
+        sys_msg_morph   := id ; 
+        sys_state_morph := id ; 
+        sys_error_morph := id ; 
+        (* coherence conditions *)
+        sys_init_coherence := sys_init_coherence_id sys ; 
+        sys_recv_coherence := sys_recv_coherence_id sys ;
+    |}.
+
+End IdentitySystemMorphism.
+
+
+(** Equality of contract morphisms *)
+Section EqualityOfSystemMorphisms.
+Context `{Serializable Setup1} `{Serializable Msg1} `{Serializable State1} `{Serializable Error1}
+        `{Serializable Setup2} `{Serializable Msg2} `{Serializable State2} `{Serializable Error2}
+        {sys1 : ContractSystem Setup1 Msg1 State1 Error1} 
+        {sys2 : ContractSystem Setup2 Msg2 State2 Error2}.
+
+Lemma eq_sm : 
+    forall (f g : SystemMorphism sys1 sys2),
+    (* if the components are equal ... *)
+    (sys_setup_morph sys1 sys2 f) = (sys_setup_morph sys1 sys2 g) -> 
+    (sys_msg_morph   sys1 sys2 f) = (sys_msg_morph   sys1 sys2 g) -> 
+    (sys_state_morph sys1 sys2 f) = (sys_state_morph sys1 sys2 g) -> 
+    (sys_error_morph sys1 sys2 f) = (sys_error_morph sys1 sys2 g) -> 
+    (* ... then the morphisms are equal *)
+    f = g.
+Proof.
+    intros f g.
+    destruct f, g.
+    cbn.
+    intros msg_eq set_eq st_eq err_eq.
+    subst.
+    f_equal;
+    apply proof_irrelevance.
+Qed.
+
+Lemma eq_sm_rev : 
+    forall (f g : SystemMorphism sys1 sys2),
+    (* if the morphisms are equal ... *)
+    f = g ->
+    (* ... then the components are equal *)
+    (sys_setup_morph sys1 sys2 f) = (sys_setup_morph sys1 sys2 g) /\
+    (sys_msg_morph   sys1 sys2 f) = (sys_msg_morph   sys1 sys2 g) /\
+    (sys_state_morph sys1 sys2 f) = (sys_state_morph sys1 sys2 g) /\
+    (sys_error_morph sys1 sys2 f) = (sys_error_morph sys1 sys2 g).
+Proof.
+    intros f g fg_eq.
+    now inversion fg_eq.
+Qed.
+
+Lemma eq_sm_iff :
+    forall (f g : SystemMorphism sys1 sys2),
+    (* the components are equal ... *)
+    (sys_setup_morph sys1 sys2 f) = (sys_setup_morph sys1 sys2 g) /\
+    (sys_msg_morph   sys1 sys2 f) = (sys_msg_morph   sys1 sys2 g) /\
+    (sys_state_morph sys1 sys2 f) = (sys_state_morph sys1 sys2 g) /\
+    (sys_error_morph sys1 sys2 f) = (sys_error_morph sys1 sys2 g) <->
+    (* ... iff the morphisms are equal *)
+    f = g.
+Proof.
+    intros.
+    split.
+    -   intro H_components.
+        destruct H_components as [H_set [H_msg [H_st H_err]]].
+        now apply eq_sm.
+    -   now apply eq_sm_rev.
+Qed.
+
+End EqualityOfSystemMorphisms.
+
+
+(** Composition of contract morphisms *)
+Section SystemMorphismComposition.
+Context `{Serializable Setup1} `{Serializable Msg1} `{Serializable State1} `{Serializable Error1}
+        `{Serializable Setup2} `{Serializable Msg2} `{Serializable State2} `{Serializable Error2}
+        `{Serializable Setup3} `{Serializable Msg3} `{Serializable State3} `{Serializable Error3}
+        { sys1 : ContractSystem Setup1 Msg1 State1 Error1} 
+        { sys2 : ContractSystem Setup2 Msg2 State2 Error2}
+        { sys3 : ContractSystem Setup3 Msg3 State3 Error3}.
+
+Lemma sys_compose_init_coh (g : SystemMorphism sys2 sys3) (f : SystemMorphism sys1 sys2) : 
+    let sys_setup_morph' := (compose (sys_setup_morph sys2 sys3 g) (sys_setup_morph sys1 sys2 f)) in 
+    let sys_state_morph' := (compose (sys_state_morph sys2 sys3 g) (sys_state_morph sys1 sys2 f)) in 
+    let sys_error_morph' := (compose (sys_error_morph sys2 sys3 g) (sys_error_morph sys1 sys2 f)) in 
+    forall c ctx s, 
+        result_functor sys_state_morph' sys_error_morph'
+            (sys_init sys1 c ctx s) = 
+        sys_init sys3 c ctx (sys_setup_morph' s).
+Proof.
+    intros.
+    unfold sys_setup_morph'.
+    cbn.
+    rewrite <- (sys_init_coherence sys2 sys3 g).
+    rewrite <- (sys_init_coherence sys1 sys2 f).
+    unfold result_functor.
+    now destruct (sys_init sys1 c ctx s).
+Qed.
+
+Lemma sys_compose_recv_coh (g : SystemMorphism sys2 sys3) (f : SystemMorphism sys1 sys2) : 
+    let sys_msg_morph'   := (compose (sys_msg_morph   sys2 sys3 g) (sys_msg_morph   sys1 sys2 f)) in 
+    let sys_state_morph' := (compose (sys_state_morph sys2 sys3 g) (sys_state_morph sys1 sys2 f)) in 
+    let sys_error_morph' := (compose (sys_error_morph sys2 sys3 g) (sys_error_morph sys1 sys2 f)) in 
+    forall c ctx st op_msg,
+        result_functor
+            (fun '(st, l) => (sys_state_morph' st, l)) sys_error_morph'
+            (sys_receive sys1 c ctx st op_msg) =
+        sys_receive sys3 c ctx (sys_state_morph' st) (option_map sys_msg_morph' op_msg).
+Proof.
+    intros.
+    pose proof (sys_recv_coherence sys2 sys3 g).
+    pose proof (sys_recv_coherence sys1 sys2 f).
+    unfold sys_state_morph', sys_msg_morph'.
+    cbn.
+    replace (option_map (compose (sys_msg_morph sys2 sys3 g) (sys_msg_morph sys1 sys2 f)) op_msg)
+    with (option_map (sys_msg_morph sys2 sys3 g) (option_map (sys_msg_morph sys1 sys2 f) op_msg)).
+    2:{ now destruct op_msg. }
+    rewrite <- H11.
+    rewrite <- H12.
+    unfold result_functor.
+    now destruct (sys_receive sys1 c ctx st op_msg).
+Qed.
+
+(** Composition *)
+Definition compose_sm (g : SystemMorphism sys2 sys3) (f : SystemMorphism sys1 sys2) :
+    SystemMorphism sys1 sys3 := {|
+    (* the components *)
+    sys_setup_morph := compose (sys_setup_morph sys2 sys3 g) (sys_setup_morph sys1 sys2 f) ; 
+    sys_msg_morph   := compose (sys_msg_morph   sys2 sys3 g) (sys_msg_morph   sys1 sys2 f) ; 
+    sys_state_morph := compose (sys_state_morph sys2 sys3 g) (sys_state_morph sys1 sys2 f) ; 
+    sys_error_morph := compose (sys_error_morph sys2 sys3 g) (sys_error_morph sys1 sys2 f) ; 
+    (* the coherence results *)
+    sys_init_coherence := sys_compose_init_coh g f ; 
+    sys_recv_coherence := sys_compose_recv_coh g f ; 
+    |}.
+
+End SystemMorphismComposition.
+
+
+(** Some results about composition *)
+Section SystemMorphismCompositionResults.
+Context `{Serializable Setup1} `{Serializable Msg1} `{Serializable State1} `{Serializable Error1}
+        `{Serializable Setup2} `{Serializable Msg2} `{Serializable State2} `{Serializable Error2}
+        `{Serializable Setup3} `{Serializable Msg3} `{Serializable State3} `{Serializable Error3}
+        `{Serializable Setup4} `{Serializable Msg4} `{Serializable State4} `{Serializable Error4}
+        {sys1 : ContractSystem Setup1 Msg1 State1 Error1} 
+        {sys2 : ContractSystem Setup2 Msg2 State2 Error2}
+        {sys3 : ContractSystem Setup3 Msg3 State3 Error3}
+        {sys4 : ContractSystem Setup4 Msg4 State4 Error4}.
+
+(** Composition with the Identity morphism is trivial *)
+Lemma compose_id_sm_left (f : SystemMorphism sys1 sys2) :
+    compose_sm (id_sm sys2) f = f.
+Proof. now apply eq_sm. Qed.
+
+Lemma compose_id_sm_right (f : SystemMorphism sys1 sys2) :
+    compose_sm f (id_sm sys1) = f.
+Proof. now apply eq_sm. Qed.
+
+(** Composition is associative *)
+Lemma compose_sm_assoc
+    (f : SystemMorphism sys1 sys2) 
+    (g : SystemMorphism sys2 sys3) 
     (h : SystemMorphism sys3 sys4) :
     compose_sm h (compose_sm g f) =
     compose_sm (compose_sm h g) f.
-Proof.
-    now apply eq_sm; unfold compose_sm; destruct f, g, h.
-Qed.
+Proof. now apply eq_sm. Qed.
 
-Definition id_sm 
-    `{ser_setup : Serializable Setup}
-    `{ser_msg : Serializable Msg}
-    `{ser_state : Serializable State}
-    (sys : ContractSystem Setup Msg State) : 
-    SystemMorphism sys sys.
-Proof.
-    apply (build_sys_morphism sys sys id id id); auto.
-    intros.
-    unfold result_functor.
-    simpl.
-    now destruct (sys_receive sys c ctx gst gmsg).
-Defined.
+End SystemMorphismCompositionResults.
 
-Definition is_iso_sm 
-    `{Serializable Setup1}
-    `{Serializable Msg1}
-    `{Serializable State1}
-    `{Serializable Setup2}
-    `{Serializable Msg2}
-    `{Serializable State2}
-    {sys1 : ContractSystem Setup1 Msg1 State1}
-    {sys2 : ContractSystem Setup2 Msg2 State2}
-    (f : SystemMorphism sys1 sys2) (g : SystemMorphism sys2 sys1) :=
-    compose_sm g f = id_sm sys1 /\
-    compose_sm f g = id_sm sys2.
 
-(** An isomorphism of contract systems *)
-Definition sys_isomorphic 
-    `{Serializable Setup1}
-    `{Serializable Msg1}
-    `{Serializable State1}
-    `{Serializable Setup2}
-    `{Serializable Msg2}
-    `{Serializable State2}
-    (sys1 : ContractSystem Setup1 Msg1 State1)
-    (sys2 : ContractSystem Setup2 Msg2 State2) : Prop := 
+Section SystemIsomorphisms.
+
+(** A bisimulation of contracts, or an isomorphism of contract traces *)
+Definition is_iso_sm
+    `{Serializable Setup1} `{Serializable Msg1} `{Serializable State1} `{Serializable Error1}
+    `{Serializable Setup2} `{Serializable Msg2} `{Serializable State2} `{Serializable Error2}
+    {sys1 : ContractSystem Setup1 Msg1 State1 Error1}
+    {sys2 : ContractSystem Setup2 Msg2 State2 Error2}
+    (m1 : SystemMorphism sys1 sys2) (m2 : SystemMorphism sys2 sys1) :=
+    compose_sm m2 m1 = id_sm sys1 /\
+    compose_sm m1 m2 = id_sm sys2.
+
+Definition systems_isomorphic
+    `{Serializable Setup1} `{Serializable Msg1} `{Serializable State1} `{Serializable Error1}
+    `{Serializable Setup2} `{Serializable Msg2} `{Serializable State2} `{Serializable Error2}
+    (sys1 : ContractSystem Setup1 Msg1 State1 Error1)
+    (sys2 : ContractSystem Setup2 Msg2 State2 Error2) :=
     exists (f : SystemMorphism sys1 sys2) (g : SystemMorphism sys2 sys1),
     is_iso_sm f g.
 
-(** E.g. if two systems have isomorphic contracts at every place, 
-    then they are isomorhpic systems *)
-Section PlaceIsomorphic.
+(* isomorphism is an equivalence relation *)
+Lemma iso_sm_refl
+    `{Serializable Setup} `{Serializable Msg} `{Serializable State} `{Serializable Error}
+    (sys : ContractSystem Setup Msg State Error) : 
+    systems_isomorphic sys sys.
+Proof.
+    exists (id_sm sys), (id_sm sys).
+    unfold is_iso_sm.
+    split; apply compose_id_sm_left.
+Qed.
 
-Record gc_iso
-    `{Serializable Setup}
-    `{Serializable Msg}
-    `{Serializable State}
-    `{Serializable Error}
-    (G1 G2 : GeneralizedContract Setup Msg State Error) := {
-    gwc_addr_iso : gc_caddr' G1 = gc_caddr' G2 ;
-    gwc_wc_iso : contracts_isomorphic (gc_c' G1) (gc_c' G2) ;
-}.
+Lemma iso_sm_sym
+    `{Serializable Setup1} `{Serializable Msg1} `{Serializable State1} `{Serializable Error1}
+    `{Serializable Setup2} `{Serializable Msg2} `{Serializable State2} `{Serializable Error2}
+    (sys1 : ContractSystem Setup1 Msg1 State1 Error1)
+    (sys2 : ContractSystem Setup2 Msg2 State2 Error2) : 
+    systems_isomorphic sys1 sys2 -> 
+    systems_isomorphic sys2 sys1.
+Proof.
+    intro sys_iso.
+    destruct sys_iso as [f [f' [f_id1 f_id2]]].
+    unfold systems_isomorphic, is_iso_sm.
+    exists f', f.
+    split.
+    -   apply f_id2.
+    -   apply f_id1.
+Qed.
 
-Definition gc_iso_op 
-    `{Serializable Setup}
-    `{Serializable Msg}
-    `{Serializable State}
-    `{Serializable Error}
-    (g1 g2 : option (GeneralizedContract Setup Msg State Error)) : Prop := 
-    match g1 with 
-    | Some G1 => 
-        match g2 with 
-        | Some G2 => gc_iso G1 G2 
-        | None => True 
-        end 
-    | None => 
-        match g2 with 
-        | Some G2 => False
-        | None => True 
-        end
-    end.
+Lemma iso_sm_trans  
+    `{Serializable Setup1} `{Serializable Msg1} `{Serializable State1} `{Serializable Error1}
+    `{Serializable Setup2} `{Serializable Msg2} `{Serializable State2} `{Serializable Error2}
+    `{Serializable Setup3} `{Serializable Msg3} `{Serializable State3} `{Serializable Error3}
+    {sys1 : ContractSystem Setup1 Msg1 State1 Error1}
+    {sys2 : ContractSystem Setup2 Msg2 State2 Error2}
+    {sys3 : ContractSystem Setup3 Msg3 State3 Error3} :
+    systems_isomorphic sys1 sys2 /\ systems_isomorphic sys2 sys3 ->
+    systems_isomorphic sys1 sys3.
+Proof.
+    intro sys_isos.
+    destruct sys_isos as [[f [f' [f_id1 f_id2]]] [g [g' [g_id1 g_id2]]]].
+    exists (compose_sm g f), (compose_sm f' g').
+    unfold is_iso_sm.
+    split.
+    -   rewrite <- compose_sm_assoc.
+        replace (compose_sm g' (compose_sm g f)) with (compose_sm (compose_sm g' g) f).
+        2:{ now rewrite <- compose_sm_assoc. }
+        rewrite g_id1.
+        rewrite compose_id_sm_left.
+        apply f_id1.
+    -   rewrite <- compose_sm_assoc.
+        replace (compose_sm f (compose_sm f' g')) with (compose_sm (compose_sm f f') g').
+        2:{ now rewrite <- compose_sm_assoc. }
+        rewrite f_id2.
+        rewrite compose_id_sm_left.
+        apply g_id2.
+Qed.
 
-(* the contracts of sys1 and sys2 are isomorphic at every place *)
-Definition sys_place_isomorphic 
-    `{Serializable Setup}
-    `{Serializable Msg}
-    `{Serializable State}
-    (sys1 : ContractSystem Setup Msg State)
-    (sys2 : ContractSystem Setup Msg State) : Prop := 
-    forall place,
-    gc_iso_op (ntree_find_node place sys1) (ntree_find_node place sys2).
-
-(* CONJECTURE <- ; we definitely want -> *)
-Proposition place_iso 
-    `{Serializable Setup}
-    `{Serializable Msg}
-    `{Serializable State} : forall
-    (sys1 : ContractSystem Setup Msg State)
-    (sys2 : ContractSystem Setup Msg State),
-    sys_place_isomorphic sys1 sys2 <->
-    sys_isomorphic sys1 sys2.
-Admitted.
-
-End PlaceIsomorphic.
-
-(** Also e.g. a permutation of the place graph leads to an isomorphism *)
-Section SystemPermutation.
-Context `{Serializable Setup} `{Serializable Msg} `{Serializable State}.
-
-Proposition sys_permute_iso : forall 
-    (sys1 : ContractSystem Setup Msg State)
-    (sys2 : ContractSystem Setup Msg State),
-    NTree_Permutation sys1 sys2 ->
-    sys_isomorphic sys1 sys2.
-Admitted.
-
-End SystemPermutation.
+End SystemIsomorphisms.
 
 End SystemMorphism.
 
 
-(** Systems of contracts can be equivalent by bisimulation *)
-Section ContractSystemEquivalence.
+Section SystemBisimulation.
 
-Section Bisimulation.
-
-(** A system's trace *)
 Section SystemTrace.
-Context `{Serializable Setup} `{Serializable Msg} `{Serializable State}.
+Context `{Serializable Msg} `{Serializable Setup} `{Serializable State} `{Serializable Error}.
 
-Record SystemStep_single
-    (sys : ContractSystem Setup Msg State)
-    (st1 st2 : SystemState State) :=
-    build_system_step_single {
-        step_chain : Chain ;
-        step_ctx : ContractCallContext ;
-        step_gmsg : SystemMsg Msg ; 
-        step_nacts : list ActionBody ;
-        (* receive is called successfully *)
-        step_recv_some : 
-            sys_receive sys step_chain step_ctx st1 step_gmsg = Ok (st2, step_nacts) ;
+(* Notions of contract state stepping forward *)
+Record SingleSystemStep (sys : ContractSystem Setup Msg State Error)
+    (prev_sys_state next_sys_state : State) :=
+    build_sys_single_step {
+    sys_step_chain : Chain ;
+    sys_step_ctx : ContractCallContext ;
+    sys_step_msg : option Msg ;
+    sys_step_nacts : list ActionBody ;
+    (* we can call receive successfully *)
+    sys_recv_ok_step :
+        sys_receive sys sys_step_chain sys_step_ctx prev_sys_state sys_step_msg =
+        Ok (next_sys_state, sys_step_nacts) ;
 }.
 
-(* in a system, a step may be one or multiple steps, chained together *)
-Definition SystemStep (sys : ContractSystem Setup Msg State) :=
-    ChainedList (SystemState State) (SystemStep_single sys).
+Definition SystemStep (sys : ContractSystem Setup Msg State Error) :=
+    ChainedList State (SingleSystemStep sys).
 
-Definition SystemTrace (sys : ContractSystem Setup Msg State) :=
-    ChainedList (SystemState State) (SystemStep sys).
+Definition SystemTrace (sys : ContractSystem Setup Msg State Error) :=
+    ChainedList State (SystemStep sys).
+
+Definition is_genesis_sys_state
+    (sys : ContractSystem Setup Msg State Error) (init_sys_state : State) : Prop :=
+    exists sys_init_chain sys_init_ctx sys_init_setup,
+    sys_init sys sys_init_chain sys_init_ctx sys_init_setup =
+    Ok init_sys_state.
+
+Definition sys_state_reachable
+    (sys : ContractSystem Setup Msg State Error) (sys_state : State) : Prop :=
+    exists init_sys_state,
+    (* init_sys_state is a valid initial sys_state *)
+    is_genesis_sys_state sys init_sys_state /\
+    (* with a trace to sys_state *)
+    inhabited (SystemTrace sys init_sys_state sys_state).
+
+Lemma inhab_trace_trans (sys : ContractSystem Setup Msg State Error) :
+forall from mid to,
+    (SystemStep sys mid to) ->
+    inhabited (SystemTrace sys from mid) ->
+    inhabited (SystemTrace sys from to).
+Proof.
+    intros from mid to step.
+    apply inhabited_covariant.
+    intro mid_t.
+    apply (snoc mid_t step).
+Qed.
 
 End SystemTrace.
 
 
-(** Morphism of system traces *)
+Section SystemTraceMorphism.
+Context `{Serializable Setup1} `{Serializable Msg1} `{Serializable State1} `{Serializable Error1}
+        `{Serializable Setup2} `{Serializable Msg2} `{Serializable State2} `{Serializable Error2}.
+
 Record SystemTraceMorphism
-    `{Serializable Setup1}
-    `{Serializable Msg1}
-    `{Serializable State1}
-    `{Serializable Setup2}
-    `{Serializable Msg2}
-    `{Serializable State2}
-    (sys1 : ContractSystem Setup1 Msg1 State1)
-    (sys2 : ContractSystem Setup2 Msg2 State2) := 
+    (sys1 : ContractSystem Setup1 Msg1 State1 Error1)
+    (sys2 : ContractSystem Setup2 Msg2 State2 Error2) := 
     build_st_morph {
-        (* state morphs, parameterized by states *)
-        st_gstate_morph : SystemState State1 -> SystemState State2 ;
-        (* some sort of init morph? *)
-        st_genesis_fixpoint : forall (init_gstate : SystemState State1),
-            is_genesis_gstate_sys sys1 init_gstate ->
-            is_genesis_gstate_sys sys2 (st_gstate_morph init_gstate) ;
-        (* step *)
-        sys_step_morph : forall gstate1 gstate2,
-            SystemStep sys1 gstate1 gstate2 -> 
-            SystemStep sys2 (st_gstate_morph gstate1) (st_gstate_morph gstate2) ;
+        (* a function *)
+        st_state_morph : State1 -> State2 ;
+        (* init state C1 -> init state C2 *)
+        sys_genesis_fixpoint : forall init_sys_state,
+            is_genesis_sys_state sys1 init_sys_state ->
+            is_genesis_sys_state sys2 (st_state_morph init_sys_state) ;
+        (* step morphism *)
+        sys_step_morph : forall sys_state1 sys_state2,
+            SystemStep sys1 sys_state1 sys_state2 ->
+            SystemStep sys2 (st_state_morph sys_state1) (st_state_morph sys_state2) ;
+        (* coherence 
+        sys_step_coh : forall from mid to step l,
+            sys_step_morph from mid step = sys_step_morph from mid step2 ->
+            sys_step_morph from to (snoc step1 l) = sys_step_morph from to (snoc step2 l) ; *)
     }.
 
-(* the identity system trace morphism *)
-Definition id_stm 
-    `{setup_ser : Serializable Setup}
-    `{msg_ser : Serializable Msg}
-    `{state_ser : Serializable State}
-    (sys : ContractSystem Setup Msg State) : SystemTraceMorphism sys sys.
+End SystemTraceMorphism.
+
+
+(** The identity trace morphism *)
+Section IdentitySTMorphism.
+Context `{Serializable Setup} `{Serializable Msg} `{Serializable State} `{Serializable Error}.
+
+Definition id_sys_genesis_fixpoint (sys : ContractSystem Setup Msg State Error) : 
+    forall init_sys_state,
+    is_genesis_sys_state sys init_sys_state ->
+    is_genesis_sys_state sys (id init_sys_state).
+Proof. auto. Defined.
+
+Definition id_sys_step_morph (sys : ContractSystem Setup Msg State Error)
+    sys_state1 sys_state2 (step : SystemStep sys sys_state1 sys_state2) :
+    SystemStep sys (id sys_state1) (id sys_state2) :=
+    step.
+
+Definition id_stm (sys : ContractSystem Setup Msg State Error) : SystemTraceMorphism sys sys := 
+{| 
+    st_state_morph := id ; 
+    sys_genesis_fixpoint := id_sys_genesis_fixpoint sys ;
+    sys_step_morph := id_sys_step_morph sys ;
+|}.
+
+End IdentitySTMorphism.
+
+
+(* Equality on system trace morphisms *)
+Section EqualityOfSTMorphisms.
+Context `{Serializable Setup1} `{Serializable Msg1} `{Serializable State1} `{Serializable Error1}
+        `{Serializable Setup2} `{Serializable Msg2} `{Serializable State2} `{Serializable Error2}.
+
+Lemma eq_stm_dep
+    (sys1 : ContractSystem Setup1 Msg1 State1 Error1)
+    (sys2 : ContractSystem Setup2 Msg2 State2 Error2)
+    (st_st_m : State1 -> State2)
+    (sys_gen_fix1 sys_gen_fix2 : forall init_sys_state,
+        is_genesis_sys_state sys1 init_sys_state ->
+        is_genesis_sys_state sys2 (st_st_m init_sys_state))
+    (sys_step_m1 sys_step_m2 : forall sys_state1 sys_state2,
+        SystemStep sys1 sys_state1 sys_state2 ->
+        SystemStep sys2 (st_st_m sys_state1) (st_st_m sys_state2)) : 
+    sys_step_m1 = sys_step_m2 ->
+    {| st_state_morph := st_st_m ;
+       sys_genesis_fixpoint := sys_gen_fix1 ;
+       sys_step_morph := sys_step_m1 ; |}
+    = 
+    {| st_state_morph := st_st_m ;
+       sys_genesis_fixpoint := sys_gen_fix2 ;
+       sys_step_morph := sys_step_m2 ; |}.
 Proof.
-    now apply (build_st_morph 
-        Setup setup_ser
-        Msg msg_ser
-        State state_ser
-        Setup setup_ser
-        Msg msg_ser
-        State state_ser
-        sys sys id).
+    intro cstep_equiv.
+    subst.
+    f_equal.
+    apply proof_irrelevance.
+Qed.
+
+End EqualityOfSTMorphisms.
+
+
+Section STMorphismComposition.
+Context `{Serializable Setup1} `{Serializable Msg1} `{Serializable State1} `{Serializable Error1}
+        `{Serializable Setup2} `{Serializable Msg2} `{Serializable State2} `{Serializable Error2}
+        `{Serializable Setup3} `{Serializable Msg3} `{Serializable State3} `{Serializable Error3}
+        {sys1 : ContractSystem Setup1 Msg1 State1 Error1}
+        {sys2 : ContractSystem Setup2 Msg2 State2 Error2}
+        {sys3 : ContractSystem Setup3 Msg3 State3 Error3}.
+
+Definition sys_genesis_compose
+    (m2 : SystemTraceMorphism sys2 sys3) (m1 : SystemTraceMorphism sys1 sys2) :
+    forall init_sys_state,
+    is_genesis_sys_state sys1 init_sys_state ->
+    is_genesis_sys_state sys3 
+        (compose (st_state_morph sys2 sys3 m2) (st_state_morph sys1 sys2 m1) init_sys_state).
+Proof.
+    destruct m2 as [smorph2 gen_fix2 step2].
+    destruct m1 as [smorph1 gen_fix1 step1].
+    intros * gen_s1.
+    now apply gen_fix1, gen_fix2 in gen_s1.
 Defined.
 
-(* composition *)
-Definition compose_stm 
-    `{ser_setup1 : Serializable Setup1}
-    `{ser_msg1 : Serializable Msg1}
-    `{ser_state1 : Serializable State1}
-    `{ser_setup2 : Serializable Setup2}
-    `{ser_msg2 : Serializable Msg2}
-    `{ser_state2 : Serializable State2}
-    `{ser_setup3 : Serializable Setup3}
-    `{ser_msg3 : Serializable Msg3}
-    `{ser_state3 : Serializable State3}
-    {sys1 : ContractSystem Setup1 Msg1 State1}
-    {sys2 : ContractSystem Setup2 Msg2 State2}
-    {sys3 : ContractSystem Setup3 Msg3 State3}
-    (m2 : SystemTraceMorphism sys2 sys3)
-    (m1 : SystemTraceMorphism sys1 sys2) :
-    SystemTraceMorphism sys1 sys3.
-Proof.
-    apply (build_st_morph 
-        Setup1 ser_setup1
-        Msg1 ser_msg1 
-        State1 ser_state1
-        Setup3 ser_setup3
-        Msg3 ser_msg3
-        State3 ser_state3
-        sys1 sys3 
-        (compose (st_gstate_morph sys2 sys3 m2) (st_gstate_morph sys1 sys2 m1))).
-    -   intros * gen_state1.
-        apply (st_genesis_fixpoint sys2 sys3 m2).
-        now apply (st_genesis_fixpoint sys1 sys2 m1).
-    -   intros * sys_step.
-        apply (sys_step_morph sys2 sys3 m2).
-        now apply (sys_step_morph sys1 sys2 m1).
-Defined.
+Definition sys_step_compose
+    (m2 : SystemTraceMorphism sys2 sys3) (m1 : SystemTraceMorphism sys1 sys2)
+    sys_state1 sys_state2 
+    (step : SystemStep sys1 sys_state1 sys_state2) :
+    SystemStep sys3 
+        (compose (st_state_morph sys2 sys3 m2) (st_state_morph sys1 sys2 m1) sys_state1) 
+        (compose (st_state_morph sys2 sys3 m2) (st_state_morph sys1 sys2 m1) sys_state2) :=
+    match m2, m1 with 
+    | build_st_morph _ _ smorph2 gen_fix2 step2, build_st_morph _ _ smorph1 gen_fix1 step1 => 
+        step2 (smorph1 sys_state1) (smorph1 sys_state2) (step1 sys_state1 sys_state2 step)
+    end.
 
-(* a strong bisimulation *)
+Definition compose_stm
+    (m2 : SystemTraceMorphism sys2 sys3) 
+    (m1 : SystemTraceMorphism sys1 sys2) : SystemTraceMorphism sys1 sys3 := 
+{| 
+    st_state_morph := compose (st_state_morph sys2 sys3 m2) (st_state_morph sys1 sys2 m1) ; 
+    sys_genesis_fixpoint := sys_genesis_compose m2 m1 ;
+    sys_step_morph := sys_step_compose m2 m1 ;
+|}.
+
+End STMorphismComposition.
+
+(** Some results on trace composition *)
+Section STMorphismCompositionResults.
+Context `{Serializable Setup1} `{Serializable Msg1} `{Serializable State1} `{Serializable Error1}
+        `{Serializable Setup2} `{Serializable Msg2} `{Serializable State2} `{Serializable Error2}
+        `{Serializable Setup3} `{Serializable Msg3} `{Serializable State3} `{Serializable Error3}
+        `{Serializable Setup4} `{Serializable Msg4} `{Serializable State4} `{Serializable Error4}
+        { sys1 : ContractSystem Setup1 Msg1 State1 Error1} 
+        { sys2 : ContractSystem Setup2 Msg2 State2 Error2}
+        { sys3 : ContractSystem Setup3 Msg3 State3 Error3}
+        { sys4 : ContractSystem Setup4 Msg4 State4 Error4}.
+
+(* Composition associative *)
+Lemma compose_stm_assoc 
+    (f : SystemTraceMorphism sys1 sys2)
+    (g : SystemTraceMorphism sys2 sys3)
+    (h : SystemTraceMorphism sys3 sys4) : 
+    compose_stm h (compose_stm g f) = 
+    compose_stm (compose_stm h g) f.
+Proof. now destruct f, g, h. Qed.
+
+(* Composition with the Identity is Trivial *)
+Lemma compose_id_stm_left (f : SystemTraceMorphism sys1 sys2) :
+    compose_stm (id_stm sys2) f = f.
+Proof. now destruct f. Qed.
+
+Lemma compose_id_stm_right (f : SystemTraceMorphism sys1 sys2) :
+    compose_stm f (id_stm sys1) = f.
+Proof. now destruct f. Qed.
+
+End STMorphismCompositionResults.
+
+(* System Bisimulations *)
+Section SystemBisimulationDefinition.
+
+(** A bisimulation of contracts, or an isomorphism of contract traces *)
 Definition is_iso_stm
-    `{Serializable Setup1}
-    `{Serializable Msg1}
-    `{Serializable State1}
-    `{Serializable Setup2}
-    `{Serializable Msg2}
-    `{Serializable State2}
-    {sys1 : ContractSystem Setup1 Msg1 State1}
-    {sys2 : ContractSystem Setup2 Msg2 State2}
+    `{Serializable Setup1} `{Serializable Msg1} `{Serializable State1} `{Serializable Error1}
+    `{Serializable Setup2} `{Serializable Msg2} `{Serializable State2} `{Serializable Error2}
+    {sys1 : ContractSystem Setup1 Msg1 State1 Error1}
+    {sys2 : ContractSystem Setup2 Msg2 State2 Error2}
     (m1 : SystemTraceMorphism sys1 sys2) (m2 : SystemTraceMorphism sys2 sys1) :=
-    compose_stm m2 m1 = id_stm sys1 /\ 
+    compose_stm m2 m1 = id_stm sys1 /\
     compose_stm m1 m2 = id_stm sys2.
 
-Section LiftingTheorem.
+Definition systems_bisimilar 
+    `{Serializable Setup1} `{Serializable Msg1} `{Serializable State1} `{Serializable Error1}
+    `{Serializable Setup2} `{Serializable Msg2} `{Serializable State2} `{Serializable Error2}
+    (sys1 : ContractSystem Setup1 Msg1 State1 Error1)
+    (sys2 : ContractSystem Setup2 Msg2 State2 Error2) :=
+    exists (f : SystemTraceMorphism sys1 sys2) (g : SystemTraceMorphism sys2 sys1),
+    (* if all steps from st to st are identified with the trivial step ... *)
+    (forall st (step : SystemStep sys1 st st), step = clnil) ->
+    (forall st (step : SystemStep sys2 st st), step = clnil) ->
+    (* ... then f and g are an isomorphism of system traces. *)
+    is_iso_stm f g.
 
-(** A morphism of systems lifts to a morphism of System Traces *)
-Definition sm_lift_stm
-    `{ser_setup1 : Serializable Setup1}
-    `{ser_msg1 : Serializable Msg1}
-    `{ser_state1 : Serializable State1}
-    `{ser_setup2 : Serializable Setup2}
-    `{ser_msg2 : Serializable Msg2}
-    `{ser_state2 : Serializable State2}
-    {sys1 : ContractSystem Setup1 Msg1 State1}
-    {sys2 : ContractSystem Setup2 Msg2 State2}
-    (f : SystemMorphism sys1 sys2) : SystemTraceMorphism sys1 sys2.
+(* bisimilarity is an equivalence relation *)
+Lemma sys_bisim_refl
+    `{Serializable Setup} `{Serializable Msg} `{Serializable State} `{Serializable Error}
+    (sys : ContractSystem Setup Msg State Error) : 
+    systems_bisimilar sys sys.
 Proof.
-    apply (build_st_morph 
-        Setup1 ser_setup1
-        Msg1 ser_msg1 
-        State1 ser_state1
-        Setup2 ser_setup2
-        Msg2 ser_msg2
-        State2 ser_state2
-        sys1 sys2 (gstate_morph sys1 sys2 f) (sys_genesis sys1 sys2 f)).
-    intros * s_step.
-    destruct f as [gstate_mph gmsg_mph gerr_mph sys_gen sys_coh].
+    exists (id_stm sys), (id_stm sys).
+    unfold is_iso_stm.
+    split; apply compose_id_stm_left.
+Qed.
+
+Lemma sys_bisim_sym
+    `{Serializable Setup1} `{Serializable Msg1} `{Serializable State1} `{Serializable Error1}
+    `{Serializable Setup2} `{Serializable Msg2} `{Serializable State2} `{Serializable Error2}
+    (sys1 : ContractSystem Setup1 Msg1 State1 Error1)
+    (sys2 : ContractSystem Setup2 Msg2 State2 Error2) : 
+    systems_bisimilar sys1 sys2 -> 
+    systems_bisimilar sys2 sys1.
+Proof.
+    intro sys_bisim.
+    unfold systems_bisimilar in *.
+    destruct sys_bisim as [f [f' triv_impl_id]].
+    exists f', f.
+    intros step_triv2 step_triv1.
+    unfold is_iso_stm in *.
+    destruct (triv_impl_id step_triv1 step_triv2) as [f_id1 f_id2].
+    split.
+    -   apply f_id2.
+    -   apply f_id1.
+Qed.
+
+Lemma iso_stm_trans
+    `{Serializable Setup1} `{Serializable Msg1} `{Serializable State1} `{Serializable Error1}
+    `{Serializable Setup2} `{Serializable Msg2} `{Serializable State2} `{Serializable Error2}
+    `{Serializable Setup3} `{Serializable Msg3} `{Serializable State3} `{Serializable Error3}
+    {sys1 : ContractSystem Setup1 Msg1 State1 Error1}
+    {sys2 : ContractSystem Setup2 Msg2 State2 Error2}
+    {sys3 : ContractSystem Setup3 Msg3 State3 Error3} :
+    systems_bisimilar sys1 sys2 /\ systems_bisimilar sys2 sys3 ->
+    (forall (st : State2) (step : SystemStep sys2 st st), step = clnil) ->
+    systems_bisimilar sys1 sys3.
+Proof.
+    intros sys_bisims step_triv2.
+    destruct sys_bisims as [[f [f' triv_impl_id_f]] [g [g' triv_impl_id_g]]].
+    unfold systems_bisimilar in *.
+    exists (compose_stm g f), (compose_stm f' g').
+    intros step_triv1 step_triv3.
+    destruct (triv_impl_id_g step_triv2 step_triv3) as [g_id1 g_id2].
+    destruct (triv_impl_id_f step_triv1 step_triv2) as [f_id1 f_id2].
+    unfold is_iso_stm.
+    split.
+    -   rewrite <- compose_stm_assoc.
+        replace (compose_stm g' (compose_stm g f)) with (compose_stm (compose_stm g' g) f).
+        2:{ now rewrite <- compose_stm_assoc. }
+        rewrite g_id1.
+        rewrite compose_id_stm_left.
+        apply f_id1.
+    -   rewrite <- compose_stm_assoc.
+        replace (compose_stm f (compose_stm f' g')) with (compose_stm (compose_stm f f') g').
+        2:{ now rewrite <- compose_stm_assoc. }
+        rewrite f_id2.
+        rewrite compose_id_stm_left.
+        apply g_id2.
+Qed.
+
+End SystemBisimulationDefinition.
+
+
+(** Contract morphisms lift to contract *trace* morphisms *)
+Section LiftingTheorem.
+Context `{Serializable Setup1} `{Serializable Msg1} `{Serializable State1} `{Serializable Error1}
+        `{Serializable Setup2} `{Serializable Msg2} `{Serializable State2} `{Serializable Error2}
+        {sys1 : ContractSystem Setup1 Msg1 State1 Error1}
+        {sys2 : ContractSystem Setup2 Msg2 State2 Error2}.
+
+Definition lift_sys_genesis (f : SystemMorphism sys1 sys2) : 
+    forall init_sys_state,
+        is_genesis_sys_state sys1 init_sys_state ->
+        is_genesis_sys_state sys2 (sys_state_morph sys1 sys2 f init_sys_state).
+Proof.
+    destruct f as [setup_morph msg_morph state_morph error_morph i_coh r_coh].
     cbn.
-    induction s_step.
-    -   apply clnil.
-    -   assert (SystemStep_single sys2 (gstate_mph mid) (gstate_mph to)) 
-        as step_single_sys2.
-        {   destruct l as [stp_chain stp_ctx stp_msg stp_nacts stp_recv].
-            apply (build_system_step_single sys2 
-                (gstate_mph mid) (gstate_mph to)
-                stp_chain 
-                stp_ctx 
-                (gmsg_mph stp_msg)
-                stp_nacts).
-            rewrite <- sys_coh.
-            now rewrite stp_recv. }
-        apply (ChainedList.snoc IHs_step step_single_sys2).
+    intros * genesis. 
+    unfold is_genesis_state in *.
+    destruct genesis as [c [ctx [s init_coh]]].
+    exists c, ctx, (setup_morph s).
+    rewrite <- i_coh.
+    unfold result_functor.
+    now destruct (sys_init sys1 c ctx s).
 Defined.
 
-(* such that id lifts to id, ... *)
-Lemma sm_lift_stm_id 
-    `{sys_set : Serializable Setup}
-    `{sys_msg : Serializable Msg}
-    `{sys_st : Serializable State}
-    {sys : ContractSystem Setup Msg State} : 
-    sm_lift_stm (id_sm sys) = id_stm sys.
+Definition lift_sys_step_morph (f : SystemMorphism sys1 sys2) : 
+    forall sys_state1 sys_state2,
+        SystemStep sys1 sys_state1 sys_state2 ->
+        SystemStep sys2 
+            (sys_state_morph sys1 sys2 f sys_state1)
+            (sys_state_morph sys1 sys2 f sys_state2).
 Proof.
-    unfold sm_lift_stm, id_sm, id_stm.
+    destruct f as [setup_morph msg_morph state_morph error_morph i_coh r_coh].
     cbn.
-    apply f_equal.
-    apply functional_extensionality_dep.
-    intro sys_state1.
-    apply functional_extensionality_dep.
-    intro sys_state2.
-    apply functional_extensionality_dep.
-    intro sys_step.
-    induction sys_step; auto.
-    destruct l.
-    cbn.
-    rewrite IHsys_step.
-    do 2 apply f_equal.
-    apply proof_irrelevance.
-Qed.
+    intros * step.
+    induction step.
+    -   apply clnil.
+    -   apply (snoc IHstep).
+        destruct l as [seq_chain seq_ctx seq_msg seq_new_acts recv_step].
+        apply (build_sys_single_step sys2 (state_morph mid) (state_morph to) 
+            seq_chain seq_ctx (option_map msg_morph seq_msg) seq_new_acts).
+        rewrite <- r_coh.
+        unfold result_functor.
+        destruct (sys_receive sys1 seq_chain seq_ctx mid seq_msg);
+        try destruct t;
+        now inversion recv_step.
+Defined.
 
-(* ... compositions lift to compositions, ... *)
-Lemma sm_lift_stm_compose 
-    `{ser_setup1 : Serializable Setup1}
-    `{ser_msg1 : Serializable Msg1}
-    `{ser_state1 : Serializable State1}
-    `{ser_setup2 : Serializable Setup2}
-    `{ser_msg2 : Serializable Msg2}
-    `{ser_state2 : Serializable State2}
-    `{ser_setup3 : Serializable Setup3}
-    `{ser_msg3 : Serializable Msg3}
-    `{ser_state3 : Serializable State3}
-    {sys1 : ContractSystem Setup1 Msg1 State1}
-    {sys2 : ContractSystem Setup2 Msg2 State2}
-    {sys3 : ContractSystem Setup3 Msg3 State3}
-    (g : SystemMorphism sys2 sys3)
-    (f : SystemMorphism sys1 sys2) : 
-    sm_lift_stm (compose_sm g f) = 
-    compose_stm (sm_lift_stm g) (sm_lift_stm f).
-Proof.
-    assert (st_gstate_morph sys1 sys3 (sm_lift_stm (compose_sm g f)) = 
-    st_gstate_morph sys1 sys3 (compose_stm (sm_lift_stm g) (sm_lift_stm f)))
-    as H_gst_eq.
-    { now destruct f, g. }
-    destruct f, g.
-    unfold compose_stm.
-    cbn in *.
-    unfold sm_lift_stm.
-    apply f_equal.
-    apply functional_extensionality_dep.
-    intro sys_state1.
-    apply functional_extensionality_dep.
-    intro sys_state2.
-    apply functional_extensionality_dep.
-    intro sys_step.
-    induction sys_step; auto.
-    destruct l.
-    cbn.
-    rewrite <- IHsys_step.
-    cbn.
-    do 2 apply f_equal.
-    apply proof_irrelevance.
-Qed.
-
-(* ... and thus isos lift to isos. *)
-Proposition sys_iso_to_st_iso 
-    `{Serializable Setup1}
-    `{Serializable Msg1}
-    `{Serializable State1}
-    `{Serializable Setup2}
-    `{Serializable Msg2}
-    `{Serializable State2}
-    {sys1 : ContractSystem Setup1 Msg1 State1} 
-    {sys2 : ContractSystem Setup2 Msg2 State2} 
-    (f : SystemMorphism sys1 sys2) (g : SystemMorphism sys2 sys1) : 
-    is_iso_sm f g -> is_iso_stm (sm_lift_stm f) (sm_lift_stm g).
-Proof.
-    intro iso_sm.
-    unfold is_iso_sm, is_iso_stm in *.
-    destruct iso_sm as [iso_sm_l iso_sm_r].
-    split.
-    -   rewrite <- sm_lift_stm_compose.
-        rewrite iso_sm_l.
-        now rewrite sm_lift_stm_id.
-    -   rewrite <- sm_lift_stm_compose.
-        rewrite iso_sm_r.
-        now rewrite sm_lift_stm_id.
-Qed.
+(** Lifting Theorem *)
+Definition sm_lift_stm (f : SystemMorphism sys1 sys2) : SystemTraceMorphism sys1 sys2 :=
+    build_st_morph sys1 sys2 
+        (sys_state_morph sys1 sys2 f) 
+        (lift_sys_genesis f) 
+        (lift_sys_step_morph f).
 
 End LiftingTheorem.
 
-End Bisimulation.
 
-End ContractSystemEquivalence.
+(** Some results on lifting *)
+Section LiftingTheoremResults.
+Context `{Serializable Setup1} `{Serializable Msg1} `{Serializable State1} `{Serializable Error1}
+        `{Serializable Setup2} `{Serializable Msg2} `{Serializable State2} `{Serializable Error2}
+        `{Serializable Setup3} `{Serializable Msg3} `{Serializable State3} `{Serializable Error3}
+        {sys1 : ContractSystem Setup1 Msg1 State1 Error1}
+        {sys2 : ContractSystem Setup2 Msg2 State2 Error2}
+        {sys3 : ContractSystem Setup3 Msg3 State3 Error3}.
+
+(** Id lifts to Id *)
+Theorem sm_lift_stm_id : 
+    sm_lift_stm (id_sm sys1) = id_stm sys1.
+Proof.
+    apply (eq_stm_dep sys1 sys1 (@id State1)).
+    apply functional_extensionality_dep.
+    intro st1.
+    apply functional_extensionality_dep.
+    intro st1'.
+    apply functional_extensionality_dep.
+    intro sys_step.
+    induction sys_step; auto.
+    unfold id_sys_step_morph in *.
+    rewrite <- IHsys_step.
+    destruct l.
+    unfold lift_sys_step_morph, id_sm, option_map.
+    cbn.
+    do 2 f_equal; auto.
+    destruct sys_step_msg0;
+    apply f_equal;
+    apply proof_irrelevance.
+Qed.
+
+(** Compositions lift to compositions *)
+Theorem sm_lift_stm_compose 
+    (g : SystemMorphism sys2 sys3) (f : SystemMorphism sys1 sys2) : 
+    sm_lift_stm (compose_sm g f) = 
+    compose_stm (sm_lift_stm g) (sm_lift_stm f).
+Proof.
+    apply (eq_stm_dep sys1 sys3 (compose (sys_state_morph sys2 sys3 g) (sys_state_morph sys1 sys2 f))).
+    apply functional_extensionality_dep.
+    intro st1.
+    apply functional_extensionality_dep.
+    intro st1'.
+    apply functional_extensionality_dep.
+    intro sys_step. 
+    induction sys_step.
+    -   destruct g as [smorph_g msgmorph_g stmorph_g errmorph_g initcoh_g recvcoh_g].
+        destruct f as [smorph_f msgmorph_f stmorph_f errmorph_f initcoh_f recvcoh_f].
+        now unfold lift_sys_step_morph.
+    -   destruct l as [s_chn s_ctx s_msg s_nacts s_recv].
+    unfold lift_sys_step_morph.
+    destruct g as [smorph_g msgmorph_g stmorph_g errmorph_g initcoh_g recvcoh_g].
+    destruct f as [smorph_f msgmorph_f stmorph_f errmorph_f initcoh_f recvcoh_f].
+    unfold option_map.
+    cbn.
+    do 2 f_equal; auto.
+    destruct s_msg;
+    apply f_equal;
+    apply proof_irrelevance.
+Qed.
+
+End LiftingTheoremResults.
+
+Section SysIsoToBisim.
+Context `{Serializable Setup1} `{Serializable Msg1} `{Serializable State1} `{Serializable Error1}
+        `{Serializable Setup2} `{Serializable Msg2} `{Serializable State2} `{Serializable Error2}
+        {sys1 : ContractSystem Setup1 Msg1 State1 Error1}
+        {sys2 : ContractSystem Setup2 Msg2 State2 Error2}.
+
+(* an isomorphism of systems lifts to a bisimulation *)
+Theorem sys_iso_to_bisim : systems_isomorphic sys1 sys2 -> systems_bisimilar sys1 sys2.
+Proof.
+    intro sys_iso.
+    destruct sys_iso as [f [g [is_iso_1 is_iso_2]]].
+    unfold systems_bisimilar.
+    exists (sm_lift_stm f), (sm_lift_stm g).
+    intros step_triv1 step_triv2.
+    clear step_triv1 step_triv2.
+    unfold is_iso_stm.
+    split.
+    -   rewrite <- sm_lift_stm_compose.
+        rewrite is_iso_1.
+        now rewrite sm_lift_stm_id.
+    -   rewrite <- sm_lift_stm_compose.
+        rewrite is_iso_2.
+        now rewrite sm_lift_stm_id.
+Qed.
+
+End SysIsoToBisim.
+
+Section LiftCMtoSM.
+Context `{Serializable Setup1} `{Serializable Msg1} `{Serializable State1} `{Serializable Error1}
+        `{Serializable Setup2} `{Serializable Msg2} `{Serializable State2} `{Serializable Error2}
+        {C1 : Contract Setup1 Msg1 State1 Error1}
+        {C2 : Contract Setup2 Msg2 State2 Error2}.
+
+Definition lift_cm_to_sm (f : ContractMorphism C1 C2) : 
+    SystemMorphism (singleton_sys C1) (singleton_sys C2).
+Proof.
+    destruct f as [setup_morph msg_morph state_morph error_morph init_coherence recv_coherence].
+    apply (build_system_morphism (singleton_sys C1) (singleton_sys C2)
+        setup_morph msg_morph state_morph error_morph);
+    unfold singleton_sys, singleton_ntree, sys_init, sys_receive, ntree_fold_left in *.
+    -   apply init_coherence.
+    -   intros.
+        rewrite <- recv_coherence.
+        cbn.
+        now destruct (receive C1 c ctx st op_msg).
+Defined.
+
+End LiftCMtoSM.
+
+Section LiftCMtoSMResults.
+Context `{Serializable Setup} `{Serializable Msg} `{Serializable State} `{Serializable Error}
+        {C : Contract Setup Msg State Error}.
+
+Lemma lift_id_cm_to_id_sm : 
+    lift_cm_to_sm (id_cm C) = id_sm (singleton_sys C).
+Proof.
+    unfold lift_cm_to_sm, id_cm, id_sm, singleton_sys.
+    cbn.
+    f_equal;
+    apply proof_irrelevance.
+Qed.
+
+Context `{Serializable Setup1} `{Serializable Msg1} `{Serializable State1} `{Serializable Error1}
+        `{Serializable Setup2} `{Serializable Msg2} `{Serializable State2} `{Serializable Error2}
+        `{Serializable Setup3} `{Serializable Msg3} `{Serializable State3} `{Serializable Error3}
+        {C1 : Contract Setup1 Msg1 State1 Error1}
+        {C2 : Contract Setup2 Msg2 State2 Error2}
+        {C3 : Contract Setup3 Msg3 State3 Error3}.
+
+Lemma lift_cm_to_sm_comp (f : ContractMorphism C1 C2) (g : ContractMorphism C2 C3) :
+    lift_cm_to_sm (compose_cm g f) = compose_sm (lift_cm_to_sm g) (lift_cm_to_sm f).
+Proof.
+    destruct g as [smorph_g msgmorph_g stmorph_g errmorph_g initcoh_g recvcoh_g].
+    destruct f as [smorph_f msgmorph_f stmorph_f errmorph_f initcoh_f recvcoh_f].
+    unfold compose_cm, compose_sm, lift_cm_to_sm.
+    cbn.
+    f_equal;
+    apply proof_irrelevance.
+Qed.
+
+
+End LiftCMtoSMResults.
+
+End SystemBisimulation.
 
 End ContractSystems.
